src/Std/Internal/Do/Order/Lemmas.lean
@@ -54,7 +54,7 @@ theorem le_of_le_bot (h : P ⊑ (⊥ : l)) : P ⊑ Q := rel_trans h (bot_le _)
 /-! ## Connectives requiring `Frame` -/
 
 section Frame
-variable [Residuated l (· ⊓ ·)]
+variable [Residuated l l (· ⊓ ·)]
 
 theorem le_himp_comm (h : P ⊓ Q ⊑ R) : P ⊑ Q ⇨ R := Residuated.le_imp (· ⊓ ·) (rel_trans meet_le_comm h)
 theorem le_himp_of_meet_le_comm (h : Q ⊓ P ⊑ R) : P ⊑ Q ⇨ R := Residuated.le_imp (· ⊓ ·) h
@@ -96,7 +96,7 @@ theorem iSup_mono {α} {Φ Ψ : α → l} (h : ∀ a, Φ a ⊑ Ψ a) : iSup Φ �
   iSup_le _ _ fun a => rel_trans (h a) (le_iSup _ a)
 
 section Frame
-variable [Residuated l (· ⊓ ·)]
+variable [Residuated l l (· ⊓ ·)]
 
 theorem himp_mono (h1 : Q ⊑ P) (h2 : P' ⊑ Q') : (P ⇨ P') ⊑ Q ⇨ Q' :=
   le_himp_comm <| rel_trans (meet_mono_right h1) <| rel_trans himp_meet_le h2
@@ -157,7 +157,7 @@ theorem bot_join : (⊥ : l) ⊔ P = P :=
 theorem join_bot : P ⊔ (⊥ : l) = P := join_comm.trans bot_join
 
 section Residuated
-variable [Residuated l (· ⊓ ·)]
+variable [Residuated l l (· ⊓ ·)]
 
 theorem meet_join_left : P ⊓ (Q ⊔ R) = (P ⊓ Q) ⊔ (P ⊓ R) :=
   rel_antisymm
@@ -261,7 +261,7 @@ theorem ofProp_forall {α} {Φ : α → Prop} :
   · exact ofProp_forall_le
 
 section Frame
-variable [Residuated l (· ⊓ ·)]
+variable [Residuated l l (· ⊓ ·)]
 
 theorem himp_ofProp_le {φ₁ φ₂ : Prop} : (⌜φ₁ → φ₂⌝ : l) ⊑ (⌜φ₁⌝ ⇨ ⌜φ₂⌝) :=
   le_himp_comm (rel_trans (rel_of_eq ofProp_and) (ofProp_mono (And.elim id)))
@@ -293,7 +293,7 @@ theorem meet_right_comm : (P ⊓ Q) ⊓ R = (P ⊓ R) ⊓ Q := by
 /-! # Working with entailment -/
 
 /-- `⊤ ⊑ (P ⇨ Q)` iff `P ⊑ Q`. -/
-@[simp] theorem top_le_himp_iff [Residuated l (· ⊓ ·)] (P Q : l) :
+@[simp] theorem top_le_himp_iff [Residuated l l (· ⊓ ·)] (P Q : l) :
     ((⊤ : l) ⊑ P ⇨ Q) ↔ (P ⊑ Q) :=
   ⟨fun h => rel_trans
     (le_meet _ _ _ (le_top _) rel_refl)
